Progress on PSS: rewriting all games using a single memory for the random oracle. Rewriting some of the proofs.

examples/PSS.ec
@@ -6,6 +6,16 @@ require import Map.
 require import Pair.
 require import Distr.
 
+(*** The belong somewhere else *)
+op pi3_1 (t:'a * 'b * 'c): 'a =
+  let (a,b,c) = t in a.
+
+op pi3_2 (t:'a * 'b * 'c): 'b =
+  let (a,b,c) = t in b.
+
+op pi3_3 (t:'a * 'b * 'c): 'c =
+  let (a,b,c) = t in c.
+
 (*** General definitions *)
 (** Lengths *)
 op k:int.
@@ -210,14 +220,12 @@ section.
   local module Mem = {
     var pk:pkey
     var sk:skey
-    var n:int
     var xstar:signature
     var qs:message set
 
-    fun init(ks:pkey*skey): unit = {
+    fun init(ks:pkey * skey): unit = {
       (pk,sk) = ks;
       qs = FSet.empty;
-      n = modulus_p pk;
       xstar = $sample_plain;
     }
   }.
@@ -352,22 +360,47 @@ section.
       first by fun; rnd; wp; skip; smt.
   qed.
 
+  (** A module to store the globals used
+      in most variants of H, along with
+      some useful equality predicates *)
+  local module Hmem = { 
+    var pk:pkey
+    var sk:skey
+    var m:(message * salt,htag * bool * signature) map
+    
+    fun init(ks:pkey*skey) : unit = { 
+      (pk,sk) = ks;
+      m = Map.empty;
+    }   
+  }.
+
+  pred (=<=) (m0:(message * salt,htag) map) (m1:(message * salt,htag * bool * signature) map) =
+    forall x, m0.[x] = if m1.[x] = None then None else Some (pi3_1 (proj m1.[x])).
+
   (** First Transition:
       We rewrite PSS into an adversary against Gen with G and a trivial split oracle H0. *)
   local module H0 : SplitOracle = { 
     fun init(ks:pkey*skey): unit = {
-      H.init();
+      Hmem.init(ks);
     }
    
     fun o(c:bool,x:message * salt):htag = { 
       var r : htag;
-      r = H.o(x);
-      return r;
+      r = $sample_htag;
+      if (!in_dom x Hmem.m) Hmem.m.[x] = (r,c,Signature.zeros);
+      return pi3_1 (proj Hmem.m.[x]);
     }
   }.
 
   local module G0 = Gen(GAdv,H0,G).
 
+  local equiv PSS_G0_H:
+    H.o ~ H0.o: ={x} /\ H.m{1} =<= Hmem.m{2} ==> ={res} /\ H.m{1} =<= Hmem.m{2}.
+  proof strict.
+  fun; inline H0.o; wp; rnd; wp; skip; rewrite /(=<=); progress=> //; smt.
+  qed.
+
+  (* More informed use of conseq* might speed up some of the smt calls *)
   local equiv PSS_G0:
     EF_CMA(Wrap(PSS(G,H)),A(G,H)).main ~ G0.main: ={glob A} ==> ={res}.
   proof strict.
@@ -378,35 +411,34 @@ section.
   inline Wrap(PSS(Gt.ROM.RO,ROM.RO)).verify PSS(Gt.ROM.RO,ROM.RO).verify
          PSS(Gt.ROM.RO,ROM.RO).g1 PSS(Gt.ROM.RO,ROM.RO).g2.
   swap{1} [18..19] -3. (* Grouping the two calls to G on the left *)
-  wp; call (_: ={glob H});
-        first by inline H0.o H.o; wp; rnd; wp; skip; smt.
+  inline GAdv(H0,Gt.ROM.RO).Hs.o; wp; call PSS_G0_H.
   (* We use seq to cut out the calls to G and limit the scope of the rcond call *)
-  wp; seq 12 11: (={glob G, glob H, w, m, maskedR, gamma} /\
+  wp; seq 12 11: (={glob G, w, m, maskedR, gamma} /\
+                  H.m{1} =<= Hmem.m{2} /\
                   Wrap.qs{1} = Mem.qs{2} /\
                   b0{1} = forged{2} /\
                   m1{1} = m{2}).
-    eqobs_in; inline Wrap(PSS(Gt.ROM.RO,ROM.RO)).init PSS(Gt.ROM.RO,ROM.RO).init
-                     ROM.RO.init Gt.ROM.RO.init PSS(Gt.ROM.RO,ROM.RO).keygen
-                     H0.init H.init Mem.init.
-    call (_: ={glob G, glob H} /\ Wrap.qs{1} = Mem.qs{2} /\ Wrap.sk{1} = Mem.sk{2}).
-     fun;eqobs_in.
-     fun;inline H0.o H.o. wp 2 5;eqobs_in.
-     fun. inline PSS(Gt.ROM.RO, ROM.RO).sign.
-       wp 9 8.
-       inline PSS(Gt.ROM.RO, ROM.RO).g1 PSS(Gt.ROM.RO, ROM.RO).g2 GAdv(H0, Gt.ROM.RO).Hs.o. 
-       eqobs_in. 
-       inline Gt.ROM.RO.o.
-       seq 12 11 : (proj Gt.ROM.RO.m.[w]{1} = g{2} /\ ={w, maskedR, ROM.RO.m, Gt.ROM.RO.m} /\ sk{1} = Mem.sk{2} /\
-                  Wrap.sk{1} = Mem.sk{2} /\ Wrap.qs{1} = Mem.qs{2} /\ (in_dom w Gt.ROM.RO.m){1}).
-          wp;rnd;wp;call (_: ={x, glob H} ==> ={res, glob H}).
-            fun;inline H.o. wp 2 3;eqobs_in.
-          wp;rnd;wp;skip;progress => //;smt.
-       wp;rnd{1};wp;skip;progress => //;smt.
-    rnd{2}; wp; rnd; wp;
-              skip; progress=> //; smt.
-    inline Gt.ROM.RO.o; rcondf{1} 9.
-      by intros=> &m //=; rnd; wp; rnd; wp; skip; progress=> //; smt.
-      by wp; rnd{1}; wp; rnd; wp; skip; progress=> //; smt.
+    wp; inline Wrap(PSS(Gt.ROM.RO,ROM.RO)).init PSS(Gt.ROM.RO,ROM.RO).init
+               ROM.RO.init Gt.ROM.RO.init PSS(Gt.ROM.RO,ROM.RO).keygen
+               H0.init H.init Mem.init.
+    call (_: ={glob G} /\ H.m{1} =<= Hmem.m{2} /\ Wrap.qs{1} = Mem.qs{2} /\ Wrap.sk{1} = Mem.sk{2}).
+     by conseq* (_: ={glob G, x} ==> ={glob G, res})=> //; fun; eqobs_in.
+     fun*; inline GAdv(H0,Gt.ROM.RO).Ha.o; sp; wp; call PSS_G0_H=> //.
+     fun; inline PSS(Gt.ROM.RO, ROM.RO).sign.
+       wp; inline PSS(Gt.ROM.RO, ROM.RO).g1 PSS(Gt.ROM.RO, ROM.RO).g2 Gt.ROM.RO.o
+                  GAdv(H0, Gt.ROM.RO).Hs.o.
+       rcondf{1} 16;
+         first by intros=> &m; inline ROM.RO.o; rnd; wp; rnd; wp; wp; rnd; wp; rnd; wp; skip; smt.
+       wp; rnd{1}; wp; rnd.
+       wp; call PSS_G0_H.
+       wp; rnd.
+       wp; skip; smt.
+    inline Hmem.init; rnd{2}; wp; rnd.
+    wp; skip; progress=> //; smt.
+
+  inline Gt.ROM.RO.o; rcondf{1} 9.
+    by intros=> &m //=; rnd; wp; rnd; wp; skip; progress=> //; smt.
+    by wp; rnd{1}; wp; rnd; wp; skip; progress=> //; smt.
   qed.        
 
   (** Second Transition:
@@ -418,26 +450,21 @@ section.
   
   axiom mu_bool_nu N p:
     2^(k - 1) <= N < 2^k =>
-     mu (bool_nu N) p =
-     (N%r - (2^(k-1))%r) / N%r * charfun p true + ((2^(k - 1))%r / N%r) * charfun p false.
+    mu (bool_nu N) p =
+      (N%r - (2^(k-1))%r) / N%r * charfun p true + ((2^(k - 1))%r / N%r) * charfun p false.
 
-  local module K = { 
-    var pk:pkey
-    var sk:skey
-    var n :int
-    
-    fun init(ks:pkey*skey) : unit = { 
-      (pk,sk) = ks;
-      n = modulus_p pk;
-    }   
-  }.
+  lemma weight_bool_nu N:
+    2^(k - 1) <= N < 2^k =>
+    weight (bool_nu N) = 1%r.
+  proof strict.
+  by intros=> bounds; rewrite /weight mu_bool_nu // /charfun /cpTrue; smt.
+  qed.
 
   local module H1: SplitOracle = {
     var bad:bool
     
     fun init(ks:pkey*skey): unit = {
-      K.init(ks);
-      H.init();
+      Hmem.init(ks);
       bad = false;
     }
 
@@ -446,106 +473,109 @@ section.
       var i:int = 0;
       var w:htag;
       w = $sample_htag;
-      if (!in_dom x H.m) {
-        H.m.[x] = HTag.zeros;
+      if (!in_dom x Hmem.m) {
         while (i < kg2 && b) {
-          b = $bool_nu K.n;
+          b = $bool_nu (modulus_p Hmem.pk);
           i = i + 1;
-          if (!b) H.m.[x] = w;
+          if (!b) Hmem.m.[x] = (w,c,Signature.zeros);
         }
       }
       bad = bad \/ b;
-      return proj H.m.[x];
+      return pi3_1 (proj Hmem.m.[x]);
     }
   }.
 
   local module G1 = Gen(GAdv,H1,G).
 
   local equiv G0_G1_H: H0.o ~ H1.o:
-    !H1.bad{2} /\ ={glob H, x} /\ 2^(k - 1) <= K.n{2} < 2^k ==>
-    !H1.bad{2} => ={glob H, res} /\ 2^(k - 1) <= K.n{2} < 2^k.
+    !H1.bad{2} /\ ={glob Hmem, x, c} /\ in_supp (Hmem.pk,Hmem.sk){2} keypairs ==>
+    in_supp (Hmem.pk,Hmem.sk){2} keypairs /\ (!H1.bad{2} => ={glob Hmem, res}).
   proof strict.
-  fun; inline H.o; case (in_dom x H.m){1}.
-    (* in_dom x H.m *)
-    rcondf{1} 3; [ | rcondf{2} 4]; first 2 by intros &m; rnd; wp.
+  fun; case (in_dom x Hmem.m){1}.
+    (* in_dom x Hmem.m *)
+    rcondf{1} 2; [ | rcondf{2} 4]; first 2 by intros &m; rnd; wp.
     by wp; rnd; wp.
 
     (* !in_dom x H.m *)
-    rcondt{1} 3; [ | rcondt{2} 4]; first 2 by intros &m; rnd; wp.
-    wp; while{2} (i <= kg2 /\ eq_except H.m{1} H.m x /\
-                  (!b => H.m.[x] = Some w{2}) /\ 2^(k - 1) <= K.n < 2^k){2} (kg2 - i){2}.
-      intros=> &m z; wp; rnd (cpTrue); skip; progress=> //; last 6 smt.
-        by rewrite mu_bool_nu // /charfun /cpTrue //=; smt.
-    by wp; rnd; wp; skip; progress=> //; smt.
+    rcondt{1} 2; [ | rcondt{2} 4]; first 2 by intros &m; rnd; wp.
+    wp; while{2} (i <= kg2 /\ eq_except Hmem.m{1} Hmem.m x /\
+                  in_supp (Hmem.pk,Hmem.sk) keypairs /\
+                  (!b => Hmem.m.[x] = Some (w,c,Signature.zeros){2})){2} (kg2 - i){2}.
+      intros=> &m z; wp; rnd (cpTrue); skip; smt.
+    by wp; rnd; wp; skip; smt.
   qed.
 
-  lemma Glossless : islossless Gt.ROM.RO.o.
-  proof. apply Gt.ROM.lossless_o;smt. qed.
+  local lemma G0_G1_abstract (Ga <: Gadv {H0,H1,G,Hmem}):
+    (forall (H <: SplitOracle {Ga}) (G <: Gt.Oracle {Ga}),
+       islossless G.o => islossless H.o => islossless Ga(H,G).main) =>
+    equiv [Gen(Ga,H0,G).main ~ Gen(Ga,H1,G).main: true ==> !H1.bad{2} => ={res}].
+  proof strict.
+  intros=> GaL; fun.
+  call (_: H1.bad,
+             ={glob G, glob Hmem} /\ in_supp (Hmem.pk,Hmem.sk){2} keypairs,
+             in_supp (Hmem.pk,Hmem.sk){2} keypairs).
+    (* G *)
+    by conseq* (_: _ ==> ={res, glob G}); last fun; eqobs_in.
+    by intros=> _ _; conseq* (_: true ==> true); first apply Gt.ROM.lossless_o; smt.
+    by intros=> _; conseq* (_: true ==> true); first apply Gt.ROM.lossless_o; smt.
+    (* H *)
+    by conseq* G0_G1_H=> //; smt.
+    by intros=> _ _; conseq* (_: true ==> true)=> //;
+         fun; wp; rnd (cpTrue); skip; smt.
+    intros=> _; fun.
+      wp; conseq* (_: _ ==> true); first smt.
+      wp; seq 3: (in_supp (Hmem.pk,Hmem.sk) keypairs)=> //;
+        first by rnd; wp; skip; smt.
+      if=> //; while (in_supp (Hmem.pk,Hmem.sk) keypairs) (kg - i).
+        by intros=> z; wp; rnd (cpTrue); skip; smt.
+      by skip; smt.
+      by conseq* (_: _ ==> false).
+  call (_: ={ks} /\ in_supp ks{2} keypairs ==>
+           ={glob Hmem} /\ !H1.bad{2} /\ in_supp (Hmem.pk,Hmem.sk){2} keypairs);
+     first by fun; wp; call (_: ={ks} /\ in_supp ks{2} keypairs ==>
+                                ={glob Hmem} /\ in_supp (Hmem.pk,Hmem.sk){2} keypairs);
+      first fun; wp.
+  call (_: true ==> ={glob G});
+    first by fun; wp.
+  by rnd; skip; smt.
+  qed.
 
   local equiv G0_G1: G0.main ~ G1.main: true ==> !H1.bad{2} => ={res}.
   proof strict.
-    apply ((_ : (forall (Ga<:Gadv{H0,H1,G,K}), 
-      (forall (H <: SplitOracle{Ga}) (G <: Gt.Oracle{Ga}),
-         islossless G.o => islossless H.o => islossless Ga(H, G).main) => 
-      equiv [Gen(Ga,H0,G).main ~ Gen(Ga,H1,G).main : true ==> !H1.bad{2} => ={res}])) GAdv).
-     intros Ga Hloosless;fun.
-     call (_: H1.bad,  (={glob G, glob H} /\ 2^(k - 1) <= K.n{2} < 2^k), (2^(k - 1) <= K.n{2} < 2^k)).
-      conseq * (_ : _ ==> ={res, glob G}) => //;fun;eqobs_in.
-      intros _ _;conseq * (_: true ==> true) => //;apply Glossless.
-      intros _;conseq * (_: true ==> true) => //;apply Glossless.
-     conseq * G0_G1_H => //.
-      intros &m1 &m2 H r1 r2 x1 x2 bad;generalize H.
-      case bad => //.
-     intros _ _;conseq * (_ : true ==> true) => //;fun.
-      call (Ht.ROM.lossless_o _) => //;smt.
-     intros _;fun.
-      wp;conseq * (_ : _ ==> true);first progress => //;smt.  
-      wp;seq 3 : (2 ^ (k - 1) <= K.n < 2 ^ k) => //.
-      rnd;wp;skip;progress => //;smt.
-      if => //.
-      while (2 ^ (k - 1) <= K.n < 2 ^ k) (kg2-i).
-       intros x;wp. conseq * (_ : _ ==> true); first progress=> //;smt.
-       rnd;skip;progress => //. 
-      by rewrite mu_bool_nu // /charfun /cpTrue //=; smt.
-      wp;skip;progress => //; smt.
-      conseq * (_: _ ==> false) => //.
-    inline Gt.ROM.RO.init H0.init H1.init H.init K.init.
-    wp;rnd;skip;progress => //;smt.
-   apply lossless_GAdv.
+  by apply (G0_G1_abstract GAdv); apply lossless_GAdv.
   qed.
+
+  (** TODO: Compute the probability of bad in {2}.
+            This requires to deal with failure events that may happen in loops. *)
 
   (** G2 *)
   local module H2 = {
     fun init(ks:pkey*skey): unit = {
-      K.init(ks);
-      H.init();
+      Hmem.init(ks);
     }
 
     fun o(c:bool, x:message * salt): htag = {
       var b:bool = true;
       var i:int = 0;
       var w:htag;
-      if (!in_dom x H.m) {
-        H.m.[x] = htag_dummy;
+      if (!in_dom x Hmem.m) {
         while (i < kg2 && b) {
-          b = $bool_nu K.n;
+          b = $bool_nu (modulus_p Hmem.pk);
           w = $sample_htag;
           i = i + 1;
-          if (!b) H.m.[x] = w;
+          if (!b) Hmem.m.[x] = (w,c,Signature.zeros);
         }
       }
-      return proj H.m.[x];
+      return pi3_1 (proj Hmem.m.[x]);
     }
   }.
 
   local module G2 = Gen(GAdv, H0, G).
 
   (** G3 *)
-
   local module H3 = {
     fun init(ks:pkey*skey): unit = {
-      K.init(ks);
-      H.init();
+      Hmem.init(ks);
     }
 
 
@@ -554,19 +584,18 @@ section.
       var i:int = 0;
       var w:htag;
       var st:gtag;
-      if (!in_dom x H.m) {
-        H.m.[x] = htag_dummy;
+      if (!in_dom x Hmem.m) {
         while (i < kg2 && b) {
-          b = $bool_nu K.n;
+          b = $bool_nu (modulus_p Hmem.pk);
           w = $sample_htag;
           i = i + 1;
           if (!b) {
-            H.m.[x] = w;
+            Hmem.m.[x] = (w,c,Signature.zeros);
             st = G.o(w);
           }
         }
       }
-      return proj H.m.[x];
+      return pi3_1 (proj Hmem.m.[x]);
     }
   }.
 
@@ -577,8 +606,7 @@ section.
     var bad:bool
 
     fun init(ks:pkey*skey): unit = {
-      K.init(ks);
-      H.init();
+      Hmem.init(ks);
       bad = false;
     }  
 
@@ -587,36 +615,32 @@ section.
       var i:int = 0;
       var w:htag;
       var st:gtag;
-      if (!in_dom x H.m) {
-        H.m.[x] = htag_dummy;
+      if (!in_dom x Hmem.m) {
         while (i < kg2 && b) {
-          b = $bool_nu K.n;
+          b = $bool_nu (modulus_p Hmem.pk);
           w = $sample_htag;
           st = $sample_gtag;
           i = i + 1;
           if (!b) {
-            H.m.[x] = w;
+            Hmem.m.[x] = (w,c,Signature.zeros);
             bad = bad \/ in_dom w G.m;
             G.m.[w] = st ^ (GTag.from_bits (to_bits (snd x) || zeros (kg - k0)));
           }
         }
       }
-      return proj H.m.[x];
+      return pi3_1 (proj Hmem.m.[x]);
     }
   }.
+
 
   local module G4 = Gen(GAdv, H4, G).
 
   (** G5 *)
-
   local module H5: SplitOracle = {
     var bad:bool
-    var m:(message * salt,htag * bool) map
 
     fun init(ks:pkey*skey): unit = {
-      K.init(ks);
-      m = Map.empty;
-      bad = false;
+      Hmem.init(ks);
     }
 
     fun o(c:bool,x:message * salt): htag = {
@@ -624,32 +648,31 @@ section.
       var i:int = 0;
       var w:htag;
       var st:gtag;
-      if (!in_dom x m) {
-        m.[x] = (htag_dummy,c);
+      if (!in_dom x Hmem.m) {
         while (i < kg2 && b) {
-          b = $bool_nu K.n;
+          b = $bool_nu (modulus_p Hmem.pk);
           w = $sample_htag;
           st = $sample_gtag;
           i = i + 1;
           if (!b) {
-            m.[x] = (w,c);
+            Hmem.m.[x] = (w,c,Signature.zeros);
             G.m.[w] = st ^ (GTag.from_bits (to_bits (snd x) || zeros (kg - k0)));
           }
         }
       } else {
-        if (!c /\ snd (proj m.[x])) {
+        if (!c /\ pi3_2 (proj Hmem.m.[x])) {
           bad = true;
-          m.[x] = (HTag.zeros,c);
+          Hmem.m.[x] = (HTag.zeros,c,Signature.zeros);
         }
       }
-      return fst (proj m.[x]);
+      return pi3_1 (proj Hmem.m.[x]);
     }
   }.
 
   local module G5 = Gen(GAdv, H5, G).
 
 (** Proofs *)
-
+(*
   pred eq_proj (m1: ('a,'b) map) (m2: ('a,'b*'c) map) = 
     forall a, in_dom a m1 = in_dom a m2 && 
      (in_dom a m1 => proj (m1.[a]) = fst (proj m2.[a])).
@@ -725,14 +748,15 @@ section.
 lemma Bad5 (A <: CMA_2RO) &m:
   Pr[G5(A(G,Ha(H5))).main() @ &m: H5.bad] <= qS%r * (qS + qH)%r/(2^k0)%r.
 admit. qed.
+*)
 
 (** G6 *)
-module H6: SplitOracle = {
+local module H6: SplitOracle = {
   var bad:bool
-  var m:(message * salt,htag * bool * signature) map
 
-  fun init(): unit = {
-    m = Map.empty;
+  fun init(ks:pkey * skey): unit = {
+    Hmem.init(ks);
+    bad = false;
   }
 
   fun o(c:bool,x:message * salt): htag = {
@@ -742,11 +766,11 @@ module H6: SplitOracle = {
     var st:gtag;
     var z, u:signature;
 
-    if (!in_dom x H.m)
+    if (!in_dom x Hmem.m)
     {
       while (i < kg2 && b)
       {
-        b = $bool_nu Mem.n;
+        b = $bool_nu (modulus_p Hmem.pk);
         w = $sample_htag;
         st = $sample_gtag;
         z = Signature.from_bits (if b then ones 1 else zeros 1 || to_bits w || to_bits st);
@@ -754,7 +778,7 @@ module H6: SplitOracle = {
         i = i + 1;
         if (!b)
         {
-          m.[x] = (w,c,u);
+          Hmem.m.[x] = (w,c,u);
           G.m.[w] = st ^ (GTag.from_bits (to_bits (snd x) || zeros (kg - k0)));
         }
       }
@@ -763,22 +787,22 @@ module H6: SplitOracle = {
     {
       if (!c) { 
         bad = true;
-        m.[x] = (HTag.zeros,c,Signature.zeros);
+        Hmem.m.[x] = (HTag.zeros,c,Signature.zeros);
       }
     }
-    return proj H.m.[x];
+    return pi3_1 (proj Hmem.m.[x]);
   }
 }.
 
-module G6 = GGen(Hs(H6),SGen(Hs(H6))).
+local module G6 = Gen(GAdv,H6,G).
 
 (** G7: No longer using sk to simulate the oracles *)
-module H7: SplitOracle = {
+local module H7: SplitOracle = {
   var bad:bool
-  var m:(message * salt,htag * bool * signature) map
 
-  fun init(): unit = {
-    m = Map.empty;
+  fun init(ks:pkey * skey): unit = {
+    Hmem.init(ks);
+    bad = false;
   }
 
   fun o(c:bool,x:message * salt): htag = {
@@ -788,7 +812,7 @@ module H7: SplitOracle = {
     var st:gtag;
     var z, u:signature;
 
-    if (!in_dom x H.m)
+    if (!in_dom x Hmem.m)
     {
       while (i < kg2 && b)
       {
@@ -800,7 +824,7 @@ module H7: SplitOracle = {
         i = i + 1;
         if (!b)
         {
-          m.[x] = (w,c,u);
+          Hmem.m.[x] = (w,c,u);
           G.m.[w] = st ^ (GTag.from_bits (to_bits (snd x) || zeros (kg - k0)));
         }
       }
@@ -808,14 +832,15 @@ module H7: SplitOracle = {
     else
     {
       bad = true;
-      if (!c) m.[x] = (HTag.zeros,c,Signature.zeros);
+      if (!c) Hmem.m.[x] = (HTag.zeros,c,Signature.zeros);
     }
-    return (lambda abc, let (a,b,c) = abc in a) (proj m.[x]);
+    return pi3_1 (proj Hmem.m.[x]);
   }
 }.
 
-module G7 = GGen(Hs(H7),SGen(Hs(H7))).
+local module G7 = Gen(GAdv,H7,G).
 
+end section.
 
 
 
@@ -896,8 +921,7 @@ module G7 = GGen(Hs(H7),SGen(Hs(H7))).
 
 
 
-
-
+(****** Old Material
 (** Proof is up to bad with BAD = (b = true) in final memory *)
 lemma equiv_G0_G1 (A <: CMA_2RO):
   equiv [G0(A(G,H)).main ~ G1(A(G,H1)).main: ={glob A} ==> !H1.bad{2} => ={res}].
@@ -1742,3 +1766,4 @@ lemma Bad1 &m:
 admit. qed.
 
 end section.
+*)
